bump to nightly-2023-04-17-18
mathlib commit https://github.com/leanprover-community/mathlib/commit/17ad94b4953419f3e3ce3e77da3239c62d1d09f0

Mathbin/Algebra/Homology/ImageToKernel.lean
@@ -46,15 +46,15 @@ theorem image_le_kernel (w : f ≫ g = 0) : imageSubobject f ≤ kernelSubobject
 /-- The canonical morphism `image_subobject f ⟶ kernel_subobject g` when `f ≫ g = 0`.
 -/
 def imageToKernel (w : f ≫ g = 0) : (imageSubobject f : V) ⟶ (kernelSubobject g : V) :=
-  Subobject.ofLe _ _ (image_le_kernel _ _ w)deriving Mono
+  Subobject.ofLE _ _ (image_le_kernel _ _ w)deriving Mono
 #align image_to_kernel imageToKernel
 
 /-- Prefer `image_to_kernel`. -/
 @[simp]
-theorem subobject_ofLe_as_imageToKernel (w : f ≫ g = 0) (h) :
-    Subobject.ofLe (imageSubobject f) (kernelSubobject g) h = imageToKernel f g w :=
+theorem subobject_ofLE_as_imageToKernel (w : f ≫ g = 0) (h) :
+    Subobject.ofLE (imageSubobject f) (kernelSubobject g) h = imageToKernel f g w :=
   rfl
-#align subobject_of_le_as_image_to_kernel subobject_ofLe_as_imageToKernel
+#align subobject_of_le_as_image_to_kernel subobject_ofLE_as_imageToKernel
 
 @[simp, reassoc.1, elementwise]
 theorem imageToKernel_arrow (w : f ≫ g = 0) :
@@ -98,7 +98,7 @@ variable [HasKernels V] [HasImages V]
 
 theorem imageToKernel_comp_right {D : V} (h : C ⟶ D) (w : f ≫ g = 0) :
     imageToKernel f (g ≫ h) (by simp [reassoc_of w]) =
-      imageToKernel f g w ≫ Subobject.ofLe _ _ (kernelSubobject_comp_le g h) :=
+      imageToKernel f g w ≫ Subobject.ofLE _ _ (kernelSubobject_comp_le g h) :=
   by
   ext
   simp
@@ -106,7 +106,7 @@ theorem imageToKernel_comp_right {D : V} (h : C ⟶ D) (w : f ≫ g = 0) :
 
 theorem imageToKernel_comp_left {Z : V} (h : Z ⟶ A) (w : f ≫ g = 0) :
     imageToKernel (h ≫ f) g (by simp [w]) =
-      Subobject.ofLe _ _ (imageSubobject_comp_le h f) ≫ imageToKernel f g w :=
+      Subobject.ofLE _ _ (imageSubobject_comp_le h f) ≫ imageToKernel f g w :=
   by
   ext
   simp
@@ -125,7 +125,7 @@ theorem imageToKernel_comp_mono {D : V} (h : C ⟶ D) [Mono h] (w) :
 @[simp]
 theorem imageToKernel_epi_comp {Z : V} (h : Z ⟶ A) [Epi h] (w) :
     imageToKernel (h ≫ f) g w =
-      Subobject.ofLe _ _ (imageSubobject_comp_le h f) ≫
+      Subobject.ofLE _ _ (imageSubobject_comp_le h f) ≫
         imageToKernel f g ((cancel_epi h).mp (by simpa using w : h ≫ f ≫ g = h ≫ 0)) :=
   by
   ext
